Lp2lc/Active/STLC/__Infer_umbralV1.lean
@@ -31,7 +31,7 @@ def infer_prove (trm : AST.Trm env.BuildParameters) (fuel : Nat) : Objective trm
     | .val (.lit _) => ⟨.yield (some ⟨.primitive⟩), rfl⟩
     | .val (.lam body tIn) =>
       let index : env.BuildParameters.B := env.uid2typCtx.inv tIn
-      let instantiated := body.specialise (AST.CarrierMap.identity _) (.inr index)
+      let instantiated := body.specialise (Parameters.CarrierMap.identity _) (.inr index)
       let result := infer_prove instantiated fuel
       ⟨result.compilation.map
           (Option.map (λ safety => ⟨.fn tIn safety.typ⟩)), by
